cache/Print.v
@@ -1,0 +1,3 @@
+From PlutusCert Require Import Language.PlutusIR.Analysis.BoundVars.
+
+Print appears_bound_in_ty_DecOpt_sound.
