src/Language/PlutusIR/Analysis/BoundVarsFast.v
@@ -1,0 +1,215 @@
+From Coq Require Import
+  Strings.String
+  Lists.List
+  Arith.PeanoNat
+  Strings.Ascii
+  Program.Basics
+  .
+
+Import ListNotations.
+Local Open Scope string_scope.
+
+From PlutusCert Require Import
+  Util
+  Util.List
+  Language.PlutusIR
+  Language.PlutusIR.Folds
+  Language.PlutusIR.Analysis.BoundVars.
+
+Import NamedTerm.
+
+From QuickChick Require Import QuickChick.
+
+
+
+
+
+Fixpoint to_names_ty (ty : Ty) : list string :=
+  match ty with
+  | Ty_Fun T1 T2 => 
+      to_names_ty T1 ++ to_names_ty T2
+  | Ty_IFix F T =>
+      to_names_ty F ++ to_names_ty T
+  | Ty_Forall X K T =>
+      X :: to_names_ty T
+  | Ty_Lam X K T =>
+      X :: to_names_ty T
+  | Ty_App T1 T2 =>
+    to_names_ty T1 ++ to_names_ty T2
+  | _ => []
+  end.
+
+(* Uses more efficient list concatination, but since the list is lazily
+ *  evaluated, I dont using this function is much faster.
+ *)
+Fixpoint to_names_ty' (ty : Ty) : list string -> list string :=
+  match ty with
+  | Ty_Fun T1 T2 => fun ls =>
+      to_names_ty' T1 (to_names_ty' T2 ls)
+  | Ty_IFix F T => fun ls =>
+      to_names_ty' F (to_names_ty' T ls)
+  | Ty_Forall X K T => fun ls =>
+      X :: to_names_ty' T ls
+  | Ty_Lam X K T => fun ls =>
+      X :: to_names_ty' T ls
+  | Ty_App T1 T2 => fun ls =>
+    to_names_ty' T1 (to_names_ty' T2 ls)
+  | _ => fun ls => ls
+  end.
+
+Lemma to_names_ty_app_equal : forall ty (xs : list string),
+  app (to_names_ty ty) xs = to_names_ty' ty xs.
+Proof.
+  induction ty; intros; simpl; auto;
+  try (rewrite <- app_assoc; rewrite IHty1; rewrite IHty2; reflexivity);
+  f_equal; apply IHty.
+Qed.
+
+Lemma to_names_ty_equal : forall ty,
+  to_names_ty ty = to_names_ty' ty [].
+Proof. intros. rewrite <- to_names_ty_app_equal. rewrite <- app_nil_end. reflexivity. Qed.
+
+
+
+(* 'accelerated' using a function evaluation, instead of a bunch of constructors defining
+ *  what it means to be 'in' a type.
+ *)
+Inductive appears_bound_in_ty' (X: tyname) (T : Ty) : Prop :=
+  | ABITYF :
+      NameIn X (to_names_ty T) ->
+      appears_bound_in_ty' X T.
+
+QCDerive DecOpt for (appears_bound_in_ty' x ty).  
+
+Instance appears_bound_in_ty'_DecOpt_sound x ty: DecOptSoundPos (appears_bound_in_ty' x ty).
+Proof. derive_sound. Qed.
+
+Instance appears_bound_in_ty'_DecOpt_complete x ty: DecOptCompletePos (appears_bound_in_ty' x ty).
+Proof. derive_complete. Qed.
+
+Instance appears_bound_in_ty'_DecOpt_monotonicity x ty: DecOptSizeMonotonic (appears_bound_in_ty' x ty).
+Proof. derive_mon. Qed.
+
+Lemma appears_bound_in_ty_in_to_name_ty : forall ty x,
+  appears_bound_in_ty x ty <-> NameIn x (to_names_ty ty).
+Proof.
+  intros ty x; split; revert x.
+  - induction ty; intros x H;
+    try (inversion H; reflexivity);
+    try (inversion H; apply NameIn_app; [left; apply IHty1 | right; apply IHty2 ]; apply H1);
+    try (inversion H; try constructor; [try apply H2 | apply IHty; apply H4 ]).
+  - induction ty; intros x H; simpl in H;
+    try (inversion H; reflexivity);
+    try (apply NameIn_app in H as [H | H];
+      [ try apply ABITY_TyFun1; try apply ABITY_TyIFix1; try apply ABITY_TyApp1; apply IHty1
+      | try apply ABITY_TyFun2; try apply ABITY_TyIFix2; try apply ABITY_TyApp2; apply IHty2 ];
+      apply H
+    );
+    try (inversion H; constructor; [ apply H2 | apply IHty; apply H3]).
+Qed.
+
+Lemma appears_bound_in_ty_equal : forall ty x, 
+  appears_bound_in_ty x ty <-> appears_bound_in_ty' x ty.
+Proof. split; intros; try constructor; apply appears_bound_in_ty_in_to_name_ty; apply H. Qed.
+
+
+
+Fixpoint bv_constructors (cs : list constructor) : list string :=
+  match cs with
+  | [] => []
+  | (Constructor (VarDecl x _) _) :: cs' => x :: bv_constructors cs'
+  end.
+
+Fixpoint to_names_tm (tm : Term) : list string :=
+  match tm with
+  | LamAbs x T t => x :: to_names_tm t
+  | Apply t1 t2 => to_names_tm t1 ++ to_names_tm t2
+  | TyAbs X K t => to_names_tm t
+  | TyInst t T => to_names_tm t
+  | IWrap F T t => to_names_tm t
+  | Unwrap t => to_names_tm t
+  | Let r bs t0 => flat_map to_names_tm_binding bs ++ to_names_tm t0
+  | _ => []
+  end
+with
+  to_names_tm_binding b := 
+    match b with 
+    | TermBind _ (VarDecl x T) t => x :: to_names_tm t
+    | DatatypeBind (Datatype XK YKs c cs) => c :: bv_constructors cs
+    | _ => []
+    end.
+
+
+Inductive appears_bound_in_tm' (x : name) : Term -> Prop :=
+  | ABITM : forall tm,
+      NameIn x (to_names_tm tm) ->
+      appears_bound_in_tm' x tm.  
+
+
+QCDerive DecOpt for (appears_bound_in_tm' x tm).
+
+Instance appears_bound_in_tm'_DecOpt_sound x tm: DecOptSoundPos (appears_bound_in_tm' x tm).
+Proof. derive_sound. Qed.
+
+Instance appears_bound_in_tm'_DecOpt_complete x ty: DecOptCompletePos (appears_bound_in_tm' x ty).
+Proof. derive_complete. Qed.
+
+Instance appears_bound_in_tm'_DecOpt_monotonicity x ty: DecOptSizeMonotonic (appears_bound_in_tm' x ty).
+Proof. derive_mon. Qed.
+
+Lemma appears_bound_in_tm_equal : forall tm x,
+  appears_bound_in_tm x tm <-> NameIn x (to_names_tm tm).
+Proof with auto using appears_bound_in_tm, NameIn.
+  intros tm x; split; revert x.
+    - induction tm; intros x H; 
+      try (inversion H; reflexivity);
+      try (induction H; simpl;
+           try rewrite <- app_assoc; 
+           try apply NameIn_app; 
+           try apply NameIn_app with (xs := _ :: _))...
+    - admit. 
+Admitted.
+
+
+
+
+
+Fixpoint to_names_ann (tm : Term) : list string :=
+  match tm with
+  | LamAbs x T tm => to_names_ty T ++ to_names_ann tm
+  | Apply tm1 tm2 => to_names_ann tm1 ++ to_names_ann tm2
+  | TyAbs X K tm => X :: to_names_ann tm
+  | TyInst tm T => to_names_ann tm ++ to_names_ty T
+  | IWrap F T tm => to_names_ty F ++ to_names_ty T ++ to_names_ann tm
+  | Unwrap t => to_names_ann t
+  | Error T => to_names_ty T
+  | Let r bs t0 => flat_map to_names_ann_binding bs ++ to_names_ann t0
+  | _ => []
+  end
+with
+  to_names_ann_binding b := 
+    match b with 
+    | TermBind sTy (VarDecl x T) t => x :: to_names_ty T ++ to_names_ann t
+    | TypeBind (TyVarDecl X K) T => X :: to_names_ty T
+    | DatatypeBind (Datatype (TyVarDecl X K) YKs c cs) => [X]
+    end.
+
+Inductive appears_bound_in_ann' (X : tyname) : Term -> Prop :=
+  | ABIA : forall tm,
+      NameIn X (to_names_ann tm) ->
+      appears_bound_in_ann' X tm.
+
+QCDerive DecOpt for (appears_bound_in_ann' x tm).
+
+Instance appears_bound_in_ann'_DecOpt_sound x tm: DecOptSoundPos (appears_bound_in_ann' x tm).
+Proof. derive_sound. Qed.
+
+Instance appears_bound_in_ann'_DecOpt_complete x tm: DecOptCompletePos (appears_bound_in_ann' x tm).
+Proof. derive_complete. Qed.
+
+Instance appears_bound_in_ann'_DecOpt_monotonic x tm: DecOptSizeMonotonic (appears_bound_in_ann' x tm).
+Proof. derive_mon. Qed.
+
+Lemma appears_bound_in_ann_in_to_name_ann : forall tm X,
+  appears_bound_in_ann X tm <-> NameIn X (to_names_ann tm).
+Proof. Admitted.
